src/dvspec/dafny/specification/consensus.dfy
@@ -32,7 +32,7 @@ module ConsensusSpec
     )
     {
         var byz := s.all_nodes - s.honest_nodes_status.Keys;
-        |byz| < f(|s.all_nodes|)
+        |byz| <= f(|s.all_nodes|)
     }
 
     predicate Init<D(!new, 0)>(
